Bring Rep relation generation up to date with Coq 8.12

theories/Glue/rep.v
@@ -22,8 +22,11 @@
   [ ] polymorphic types like [option]
   [ ] multi-polymorphic types like [pair]
   [ ] recursive and polymorphic types like [list]
-  [ ] recursive and dependent types like [vector]
-  [ ] types of sort Prop like [and] or [le]
+  [ ] recursive and dependent types like [fin]
+  [ ] recursive, polymorphic and dependent types like [vector]
+  [ ] nested types
+  [ ] types of sort Prop like [True], [and] or [le]
+  [ ] types that use functions in its definition
 
   Game plan:
   * Take a type constructor (in Coq, not reified) as an input.
@@ -36,7 +39,14 @@
       quantify over all parameters and indices.
   * If a block is missing any instance,
     define type class instances for each type in the block.
+
+  Caveats:
+  * If a type is of sort [Prop], the representation of its values is
+    the same as [unit] for all vallues.
+  * Parameters are not included in the memory representation,
+    indices are. But parameters should be quantified over in the [Rep] instance type.
 *)
+
 Require Import Coq.ZArith.ZArith
                Coq.Program.Basics
                Coq.Strings.String
@@ -53,7 +63,24 @@ Require Import MetaCoq.Template.All.
 
 Require Import glue_utils.
 
+(* Warning: MetaCoq doesn't use the Monad notation from ExtLib,
+  therefore don't expect ExtLib functions to work with TemplateMonad. *)
+Import monad_utils.MonadNotation
+       ListNotations
+       MetaCoqNotations.
+
+Check <%% list nat %%>.
 Require CertiCoq.L6.Prototype.
+(* Alias to distinguish terms that are NOT in de Bruijn notation. *)
+Definition named_term : Type := term.
+(* Alias for terms that do not contain references to local variables,
+   therefore can be used in either [term]s in de Bruijn notation
+   and [named_term]s in named notation. *)
+Definition global_term : Type := term.
+(* Alias to denote that a function works with
+   either [term], [named_term] or [global_term]. *)
+Definition any_term : Type := term.
+
 Module DB.
   (* Uses code written by John Li.
      We should eventually consider making a MetaCoq_utils module. *)
@@ -67,36 +94,80 @@ Module DB.
 
   (* Takes a named representation, which we hack by using names starting with $,
      and converts it into the de Bruijn representation. *)
-  Definition deBruijn (t : term) : TemplateMonad term :=
+  Definition deBruijn (t : named_term) : TemplateMonad term :=
     runGM (indices_of [] t).
 
   (* Example usage for deBruijn:
 
-     MetaCoq Run (t <- DB.deBruijn <% fun (x : bool) => x %> ;;
+     MetaCoq Run (t <- DB.deBruijn
+                          (tLambda (nNamed "$x") <% bool %> (tVar "$x")) ;;
+                  t' <- tmUnquoteTyped (bool -> bool) t ;;
                   tmPrint t).
   *)
 
   (* Takes a de Bruijn representation and adds $ to local variables,
      and changes [tRel]s to [tVar]s referring to those variabstarting with $. *)
-  Definition undeBruijn (initial : list ident) (t : term) : TemplateMonad term :=
+  Definition undeBruijn (initial : list ident)
+                        (t : term) : TemplateMonad named_term :=
     runGM (named_of initial t).
 
   (* Example usage for undeBruijn:
 
-     MetaCoq Run (t <- DB.undeBruijn nil (tLambda (nNamed "$x") <% bool %> (tVar "$x")) ;;
-                  t' <- tmUnquoteTyped (bool -> bool) t ;;
-                  tmPrint t).
   *)
+     MetaCoq Run (t <- DB.undeBruijn nil <% fun (x : bool) => x %> ;;
+                  tmPrint t).
 End DB.
 
-(* Warning: MetaCoq doesn't use the Monad notation from ExtLib,
-  therefore don't expect ExtLib functions to work with TemplateMonad. *)
-Import monad_utils.MonadNotation
-       ListNotations
-       MetaCoqNotations.
+
+Module Substitution.
+  (* Capturing substitution for named terms, only use for global terms. *)
+  Fixpoint named_subst (t : global_term) (x : ident) (u : named_term) {struct u} : named_term :=
+    match u with
+    | tVar id => if eq_string id x then t else u
+    | tEvar ev args => tEvar ev (map (named_subst t x) args)
+    | tCast c kind ty => tCast (named_subst t x c) kind (named_subst t x ty)
+    | tProd (mkBindAnn (nNamed id) rel) A B =>
+      if eq_string x id
+      then tProd (mkBindAnn (nNamed id) rel) (named_subst t x A) B
+      else tProd (mkBindAnn (nNamed id) rel) (named_subst t x A) (named_subst t x B)
+    | tProd na A B => tProd na (named_subst t x A) (named_subst t x B)
+    | tLambda (mkBindAnn (nNamed id) rel) T M =>
+      if eq_string x id
+      then tLambda (mkBindAnn (nNamed id) rel) (named_subst t x T) M
+      else tLambda (mkBindAnn (nNamed id) rel) (named_subst t x T) (named_subst t x M)
+    | tLambda na T M => tLambda na (named_subst t x T) (named_subst t x M)
+    | tLetIn (mkBindAnn (nNamed id) rel) b ty b' =>
+      if eq_string x id
+      then tLetIn (mkBindAnn (nNamed id) rel) (named_subst t x b) (named_subst t x ty) b'
+      else tLetIn (mkBindAnn (nNamed id) rel) (named_subst t x b) (named_subst t x ty) (named_subst t x b')
+    | tLetIn na b ty b' => tLetIn na (named_subst t x b) (named_subst t x ty) (named_subst t x b')
+    | tApp u0 v => mkApps (named_subst t x u0) (map (named_subst t x) v)
+    | tCase ind p c brs =>
+        let brs' := map (on_snd (named_subst t x)) brs in
+        tCase ind (named_subst t x p) (named_subst t x c) brs'
+    | tProj p c => tProj p (named_subst t x c)
+    | tFix mfix idx => (* FIXME *)
+      let mfix' := map (map_def (named_subst t x) (named_subst t x)) mfix in
+      tFix mfix' idx
+    | tCoFix mfix idx =>
+      let mfix' := map (map_def (named_subst t x) (named_subst t x)) mfix in
+      tCoFix mfix' idx
+    | _ => u
+    end.
+
+  (* Substitute multiple [global_term]s into a [named_term]. *)
+  Fixpoint named_subst_all (l : list (ident * global_term)) (u : named_term) : named_term :=
+    match l with
+    | nil => u
+    | (id, t) :: l' => named_subst_all l' (named_subst t id u)
+    end.
+End Substitution.
 
 Notation "f >=> g" := (fun x => (f x) >>= g)
                       (at level 51, right associativity) : monad_scope.
+Notation "f <$> x" := (x' <- x%monad ;; ret (f x'))
+                      (at level 52, right associativity) : monad_scope.
+Open Scope string.
 
 Variables (graph : Type) (mtype : Type).
 
@@ -109,76 +180,128 @@ Variable fitting_index : graph -> mtype -> cRep -> list mtype -> Prop.
 Class Rep (A : Type) : Type :=
   { rep : forall (g : graph) (x : A) (p : mtype), Prop }.
 
-
 (* Starting generation of [Rep] instances! *)
 
-(* (* Possibly useful code: *)
+Section Argumentation.
 
-Record TypeCtorInfo :=
-  { type_ctor_kername : kername
-  ; type_ctor_inductive : inductive
-  ; type_ctor_term : term
-  }.
+  Variant arg_variant : Type :=
+  | param_arg : forall (param_name : ident) (param_type : named_term), arg_variant
+  | value_arg : forall (arg_name exists_name : ident) (arg_type : named_term), arg_variant.
 
-Definition getTypeCtor {kind : Type} (T : kind) : TemplateMonad TypeCtorInfo :=
-  '(env, t) <- tmQuoteRec T ;;
-  match t with
-  | tInd ind _ =>
-    let first_kn := inductive_mind ind in
-    match lookup first_kn env with
-    | Some (InductiveDecl mut) =>
-      match nth_error (ind_bodies mut) (inductive_ind ind) with
-      | None =>
-        tmFail ("Could not find #" ++ string_of_nat (inductive_ind ind)
-                ++ " in the mutual type block of " ++ string_of_kername first_kn)
-               (* this should never happen *)
-      | Some one =>
-        ret {| type_ctor_kername := (fst first_kn, ind_name one)
-             ; type_ctor_inductive := ind
-             ; type_ctor_term := t
-             |}
-      end
-    | _ =>
-      tmFail ("Could not find the inductive declaration for "
-              ++ string_of_kername first_kn ++ " in the type environment")
-             (* this should never happen *)
-    end
-  | _ =>
-    tmPrint T ;; tmFail "is not an inductive type constructor."
-  end.
+  (* Takes the identifying information for a single inductive type
+     in a mutual block, a constructor for that type,
+     and generates the list of arguments and the [named_term]
+     that is possibly using those argument names. *)
+  Definition argumentation
+             (ind : inductive)
+             (mut : mutual_inductive_body)
+             (ctor : ctor_info) : TemplateMonad (list arg_variant * named_term) :=
+    let number_of_params : nat := ind_npars mut in
+    (* The type names are referred with de Bruijn indices
+       so we must add them to the initial context. *)
+    let mp : modpath := fst (inductive_mind ind) in
+    let kn : kername := inductive_mind ind in
+    (* We need two passes here,
+       - one to replace the type references to globally unique [ident]s
+       - another to substitute those [ident]s into terms referring to those types,
+         so that later when we encounter the [tInd] we know which [Rep] instance to call.
+     *)
+    let mut_names : list ident :=
+        map (fun one => "$$$" ++ string_of_kername (mp, ind_name one)) (ind_bodies mut) in
+    let mut_ind_terms : list (ident * global_term) :=
+        mapi (fun i one =>
+                let id := "$$$" ++ string_of_kername (mp, ind_name one) in
+                let ind := mkInd kn i in
+                (id, tInd ind nil))
+            (ind_bodies mut) in
 
-MetaCoq Run (getTypeCtor term).
+    let fix aux (params : nat) (* number of parameters left *)
+                (arg_count : nat) (* number of args seen *)
+                (ctx : list ident) (* names of params and args to be used *)
+                (t : term) (* what is left from the constructor type *)
+                {struct t}
+                : TemplateMonad (list arg_variant * named_term) :=
+      match params, t with
+      (* Go through the params *)
+      | S params', tProd n t b =>
+        match n with
+        | mkBindAnn (nNamed id) _ =>
+          let id := "$" ++ id in (* as our naming hack requires *)
+          '(args, rest) <- aux params' arg_count (id :: ctx) b ;;
+          t' <- DB.undeBruijn ctx t ;;
+          let t' := Substitution.named_subst_all mut_ind_terms t' in
+          ret (param_arg id t' :: args, rest)
+        | _ => tmFail "Impossible: unnamed param"
+        end
+      | S _ , _ => tmFail "Impossible: all constructors quantify over params"
+
+      (* Other arguments *)
+      | O , tProd n t b =>
+        let arg_name : ident := "$arg" ++ string_of_nat arg_count in
+        let exists_name : ident := "$p" ++ string_of_nat arg_count in
+        '(args, rest) <- aux O (S arg_count) (arg_name :: ctx) b ;;
+        t' <- DB.undeBruijn ctx t ;;
+        let t' := Substitution.named_subst_all mut_ind_terms t' in
+        ret (value_arg arg_name exists_name t' :: args, rest)
+      | O, t =>
+        (* rename variables in the root *)
+        t' <- DB.undeBruijn ctx t ;;
+        let t' := Substitution.named_subst_all mut_ind_terms t' in
+        ret (nil , t')
+      end in
+
+    aux number_of_params O mut_names (ctor_type ctor).
+
+End Argumentation.
+
+Definition is_sort : Type := bool.
+
+(* Takes the identifying information for a single inductive type
+   in a mutual block, and generates a type for the whole block.
+   This is a function that will be used to generate the type of the new [Rep] instance,
+   for which the [type_quantifier] adds a [Rep] instance argument.
+   This function can also be used to get a fully applied [named_term] and its quantifiers.
+   The quantifiers would go around the [rep] function and the [Rep] instance.
 *)
-
 Definition generate_instance_type
            (ind : inductive)
            (one : one_inductive_body)
-           (replacer : term -> term) : TemplateMonad term :=
+           (type_quantifier : ident -> named_term -> named_term)
+           (replacer : named_term -> named_term) : TemplateMonad named_term :=
   (* Convert the type of the type to explicitly named representation *)
   ty <- DB.undeBruijn [] (ind_type one) ;;
+  let check_sort (t : any_term) : is_sort :=
+      match t with tSort _ => true | _ => false end in
   (* Goes over a nested π-type and collects binder names,
      makes up a name where there isn't one.
      It also builds a function to replace the part after the π-binders. *)
   let fix collect
-          (t : term) (count : nat) (replacer : term -> term)
-          : list ident * (term -> term) :=
+          (t : named_term) (count : nat) (replacer : named_term -> named_term)
+          : list (ident * is_sort) * (named_term -> named_term) :=
     match t with
-    | tProd nAnon ty rest =>
+    | tProd (mkBindAnn nAnon rel) ty rest =>
         let '(idents, f) := collect rest (S count) replacer in
-        let new_name := "$arg" ++ string_of_nat count in
-        (new_name :: idents, (fun t' => tProd (nNamed new_name) ty (f t')))
-    | tProd (nNamed id) ty rest =>
+        let new_name := "$P" ++ string_of_nat count in
+        ((new_name, check_sort ty) :: idents, (fun t' => tProd (mkBindAnn (nNamed new_name) rel) ty (f t')))
+    | tProd (mkBindAnn (nNamed id) rel) ty rest =>
         let '(idents, f) := collect rest (S count) replacer in
-        (id :: idents, (fun t' => tProd (nNamed id) ty (f t')))
+        ((id, check_sort ty) :: idents, (fun t' => tProd (mkBindAnn (nNamed id) rel) ty (f t')))
     | _ => (nil, replacer)
     end in
-  let (names, new) := collect ty 0 replacer in
+  let (quantified, new) := collect ty 0 replacer in
+  let names := map fst quantified in
   let vars := map tVar names in
+  let type_quantifiers := map fst (filter snd quantified) in
+  let base := tApp (tInd ind []) vars in
+
   (* Fully apply the quantified type constructor.
      If you had [list] initially, now you have [forall (A : Type), list A] *)
-  let result := new (tApp (tInd ind []) vars) in
+  let result := new (fold_right type_quantifier base type_quantifiers) in
+  ret result.
   (* Convert back to de Bruijn notation and return. *)
-  DB.deBruijn result.
+  (* We should use [deBruijn] here because [undeBruijn]ing adds
+     a number and $ to every name, which is useless to us later. *)
+  (* DB.deBruijn result. *)
 
 (* Checks if the given type class instance type has an instance.
    This wrapper function makes type checking easier
@@ -187,14 +310,22 @@ Definition has_instance (A : Type) : TemplateMonad bool :=
   opt_ins <- tmInferInstance (Some all) A ;;
   ret (match opt_ins with | my_Some _ => true | my_None => false end).
 
+Definition generate_Rep_instance_type
+           (ind : inductive)
+           (one : one_inductive_body) : TemplateMonad named_term :=
+  generate_instance_type ind one
+    (fun ty_name t =>
+      let n := "$Rep_" ++ Prototype.remove_sigils' ty_name in
+      tProd (mkBindAnn (nNamed n) Relevant) (tApp <% Rep %> [tVar ty_name]) t)
+    (fun t => tApp <% Rep %> [t]).
+
 (* Constructs the instance type for the type at hand,
    checks if there's an instance for it. *)
 Definition find_missing_instance
            (ind : inductive)
            (one : one_inductive_body) : TemplateMonad bool :=
-  t <- generate_instance_type ind one (fun t => tApp <% Rep %> [t]) ;;
-  t' <- tmUnquoteTyped Type t ;;
-  has_instance t'.
+  generate_Rep_instance_type ind one >>=
+  DB.deBruijn >>= tmUnquoteTyped Type >>= has_instance.
 
 (* Take in a [global_env], which is a list of declarations,
    and find the inductive declarations in that list
@@ -215,85 +346,95 @@ Fixpoint find_missing_instances
     | nil => ret nil
     end.
 
+Definition get_ty_info_from_inductive
+           (ind : inductive) : TemplateMonad ty_info :=
+  mut <- tmQuoteInductive (inductive_mind ind) ;;
+  match nth_error (ind_bodies mut) (inductive_ind ind) with
+  | None => tmFail "Wrong index for the mutual inductive block"
+  | Some one =>
+      params <- monad_map (fun c => match decl_name c with
+                           | mkBindAnn nAnon _ => tmFail "Unnamed inductive type parameter"
+                           | mkBindAnn (nNamed n) _ => ret n
+                           end) (ind_params mut) ;;
+      ret {| ty_name := inductive_mind ind
+           ; ty_body := one
+           ; ty_inductive := ind
+           ; ty_params := params
+           |}
+  end.
+
+(* Get the [ty_info] for the first type in the mutual block. *)
+Definition get_ty_info
+           (kn : kername) : TemplateMonad ty_info :=
+  get_ty_info_from_inductive {| inductive_mind := kn ; inductive_ind := 0 |}.
+
+Definition get_one_from_inductive
+           (ind : inductive) : TemplateMonad one_inductive_body :=
+  ty_body <$> get_ty_info_from_inductive ind.
 
 
-
-Record arg_info : Type :=
-  { arg_name : BasicAst.ident
-    (* the bound name used in the constructor, inside the pattern *)
-  ; p_name : BasicAst.ident
-    (* the bound name used in the exists *)
-  ; arg_type : term
-    (* the term for the main inductive type used *)
-    (* TODO think about the fully applied type for polymorphic/dependent types *)
-  ; arg_inductive : inductive
-    (* the name of the type constructor used in the argument, like [nat], [list], [option] *)
-  }.
-
-Fixpoint handle_dissected_args
-         (args : list dissected_type)
-         (count : nat)
-          : TemplateMonad (list arg_info) :=
-    match args with
-    | nil => ret nil
-    | cons (dInd ind) args' =>
-      rest <- handle_dissected_args args' (S count) ;;
-      let arg_s : BasicAst.ident := ("$arg" ++ string_of_nat count)%string in
-      let ex_s : BasicAst.ident := ("$p" ++ string_of_nat count)%string in
-      let t : term := tInd ind nil in
-      ret ({| arg_name := arg_s
-            ; p_name := ex_s
-            ; arg_type := t
-            ; arg_inductive := ind |} :: rest)
-    | cons decl _ =>
-      tmPrint decl ;;
-      tmFail "Dissected type is not a type"
-    end.
+Definition make_tInd (ind : inductive) : global_term :=
+  tInd ind [].
 
 Fixpoint make_lambdas
-         (args : list arg_info)
-         : term -> term :=
+         (args : list arg_variant)
+         : named_term -> named_term :=
   match args with
-  | nil => fun x => x
-  | arg :: args' =>
-    fun x => tLambda (nNamed (arg_name arg))
-                     (arg_type arg)
+  | value_arg arg_name _ nt :: args' =>
+    fun x => tLambda (mkBindAnn (nNamed arg_name) Relevant)
+                     nt
                      (make_lambdas args' x)
+  | _ :: args' => fun x => make_lambdas args' x
+  | _ => fun x => x
   end.
 
 Fixpoint make_exists
-         (args : list arg_info)
-         : term -> term :=
+         (args : list arg_variant)
+         : named_term -> named_term :=
   match args with
-  | nil => fun x => x
-  | arg :: args' =>
+  | value_arg _ p_name nt :: args' =>
     fun x => tApp <% ex %>
                   [ <% mtype %>
-                  ; tLambda (nNamed (p_name arg))
+                  ; tLambda (mkBindAnn (nNamed p_name) Relevant)
                             <% mtype %>
                             (make_exists args' x) ]
+  | _ => fun x => x
   end.
 
 
-Definition t_cons (t : term) (t' : term) : term :=
+(* Special helper functions to make lists consisting of [mtype] values *)
+Definition t_cons (t : any_term) (t' : any_term) : any_term :=
   tApp <% @cons %> [<% mtype %> ; t ; t'].
-Definition t_conses (xs : list term) : term :=
+Definition t_conses (xs : list any_term) : any_term :=
   fold_right t_cons <% @nil mtype %> xs.
-Definition t_and (t : term) (t' : term) : term :=
+Definition t_and (t : any_term) (t' : any_term) : any_term :=
   tApp <% @and %> [t ; t'].
 
-Print one_inductive_body.
-Compute (seq 0 4).
+(* [tmInferInstance] can create some type checking error
+   but this definition solves it for some reason. *)
+Definition tmInferInstanceEval (t : Type) := tmInferInstance (Some all) t.
+
+(* Takes in a term representing a type like [forall A, Rep (list A)])
+
+*)
+Definition instance_term (inst_ty : term) : TemplateMonad global_term :=
+  inst_ty' <- tmUnquoteTyped Type inst_ty ;;
+  opt_ins <- tmInferInstanceEval inst_ty' ;;
+  match opt_ins with
+  | my_Some x => tmQuote x
+  | _ => tmFail "No such instance"
+  end.
+
 Fixpoint make_prop
          (ind : inductive)
          (one : one_inductive_body)
          (ctor : ctor_info)
-         (args : list arg_info)
-         : TemplateMonad term :=
+         (args : list arg_variant)
+         : TemplateMonad named_term :=
   let t_g := tVar "$g" in
   let t_p := tVar "$p" in
 
-  let make_prop_base : TemplateMonad term :=
+  let make_prop_base : TemplateMonad named_term :=
     (* Create the [cRep] for this constructor and evaluate *)
     crep <- tmEval all
               (match ctor_arity ctor with
@@ -308,35 +449,61 @@ Fixpoint make_prop
               [ t_g ; t_p ; t_crep ; l])
   in
 
-  (* Takes in the order of the argument and the [arg_info], *)
-(*      generates the call to [rep] for that argument *)
-  let make_arg_prop (arg' : nat * arg_info) : TemplateMonad term :=
-    let '(i, arg) := arg' in
-    let t_arg := tVar ("$arg" ++ string_of_nat i) in
-    let t_p := tVar ("$p" ++ string_of_nat i) in
-
-    (* Check if this is a recursive call to the [rep] we're defining *)
-    if eq_inductive ind (arg_inductive arg)
-    then
-      let t_rep := tVar ("$rep_" ++ ind_name one) in
-      ret (tApp t_rep [ t_g ; t_arg; t_p ])
-    else
-      (* not a recursive call, find the right [Rep] instance *)
-      ty <- tmUnquoteTyped Type (arg_type arg) ;;
-      opt_ins <- tmInferInstance (Some all) (Rep ty) ;; (* FIXME polymorphic *)
-      match opt_ins with
-      | my_Some ins =>
-        t_ins <- tmQuote ins ;;
-        ret (tApp <% @rep %> [ arg_type arg ; t_ins ; t_g ; t_arg; t_p ])
-      | my_None =>
-          tmFail ("No instance found")
+  let named_term_root (nt : named_term) : TemplateMonad inductive :=
+      tmMsg "named_term_root:" ;;
+      tmEval all nt >>= tmPrint ;;
+      match nt with
+      | tInd ind _ | tApp (tInd ind _) _ => ret ind
+      | _ => tmFail ("Cannot find root of the argument term: " ++ string_of_term nt)
       end
   in
-  arg_props <- monad_map make_arg_prop (enumerate_nat args) ;;
+
+  let fix build_rep_call (nt : named_term) : TemplateMonad named_term :=
+      tmMsg "build_rep_call:" ;;
+      tmEval all nt >>= tmPrint ;;
+      match nt with
+      | tInd arg_inductive _ =>
+        if eq_kername (inductive_mind ind) (inductive_mind arg_inductive)
+        then ret (tVar ("$rep" ++ string_of_nat (inductive_ind arg_inductive)))
+        else
+          one <- get_one_from_inductive arg_inductive ;;
+          (* not a recursive call, find the right [Rep] instance *)
+          inst_ty <- generate_Rep_instance_type arg_inductive one ;;
+          tmMsg "Finding Rep instance for the type:" ;;
+          tmEval all inst_ty >>= tmPrint ;;
+          (* TODO fix this for special [Rep] instances *)
+          t_ins <- instance_term inst_ty ;;
+          (* TODO construct applications to the t_ins *)
+          ret (tApp <% @rep %> [ make_tInd arg_inductive ; t_ins ])
+      | tApp root args => (* TODO fix args *)
+          build_rep_call root
+      | tVar ty_name => ret (tVar ("$Rep_" ++ Prototype.remove_sigils' ty_name))
+      | _ => tmFail ("Cannot find root of the argument term: " ++ string_of_term nt)
+      end
+  in
+
+  (* Takes in the [arg_variant],
+     generates the call to [rep] for that argument.
+     Returns a list so that [param_arg] can return a empty list. *)
+  let make_arg_prop (arg : arg_variant) : TemplateMonad (list named_term) :=
+    match arg with
+      | value_arg arg_name p_name nt =>
+        tmMsg "HERE'S ONE!" ;;
+        let t_arg := tVar arg_name in
+        let t_p := tVar p_name in
+        call <- build_rep_call nt ;;
+        ret [tApp call [ t_g ; t_arg; t_p ]]
+      | _ => ret nil
+    end
+  in
+  arg_props <- monad_map make_arg_prop args ;;
+  tmMsg "arg_props:" ;;
+  tmEval all arg_props >>= tmPrint ;;
   base <- make_prop_base ;;
-  ret (fold_right t_and base arg_props).
+  ret (fold_right t_and base (concat arg_props)).
 
-
+(* Takes in the info for a single constructor of a type, generates the branches
+   of a match expression for that constructor. *)
 Definition ctor_to_branch
     (ind : inductive)
       (* the type we're generating for *)
@@ -346,11 +513,19 @@ Definition ctor_to_branch
       (* reified term of the type we're generating for *)
     (ctor : ctor_info)
       (* a single constructor to generate for *)
-    : TemplateMonad (nat * term) :=
-  let '(dissected_args, dissected_res) :=
-      (* FIXME params *)
-      dissect_types nil (dInd ind :: nil) (ctor_type ctor) in
-  args <- handle_dissected_args dissected_args O ;;
+    : TemplateMonad (nat * named_term) :=
+  let kn : kername := inductive_mind ind in
+  mut <- tmQuoteInductive kn ;;
+  let ctx : list dissected_type :=
+      mapi (fun i _ => dInd {| inductive_mind := kn ; inductive_ind := i |})
+           (ind_bodies mut) in
+  params <- ty_params <$> get_ty_info (inductive_mind ind) ;;
+  mut <- tmQuoteInductive (inductive_mind ind) ;;
+  '(args, res) <- argumentation ind mut ctor ;;
+
+  tmMsg "ARGS:" ;;
+  tmEval all args >>= tmPrint ;;
+
   prop <- make_prop ind one ctor args ;;
   let t := make_lambdas args (make_exists args prop) in
   ret (ctor_arity ctor, t).
@@ -365,10 +540,10 @@ Definition matchmaker
       (* reified term of the type we're generating for *)
     (ctors : list ctor_info)
       (* constructors we're generating match branches for *)
-    : TemplateMonad term :=
+    : TemplateMonad named_term :=
   branches <- monad_map (ctor_to_branch ind one tau) ctors ;;
-  ret (tCase (ind, 0)
-             (tLambda (nNamed "$y"%string) tau <% Prop %>)
+  ret (tCase (ind, 0, Relevant)
+             (tLambda (mkBindAnn (nNamed "$y") Relevant) tau <% Prop %>)
              (tVar "$x")
              branches).
 
@@ -379,45 +554,50 @@ Definition matchmaker
 Definition make_fix_single
            (tau : term) (* fully applied type constructor *)
            (ind : inductive)
-           (one : one_inductive_body) : TemplateMonad (BasicAst.def term) :=
-  let this_name := nNamed ("$rep_" ++ ind_name one)%string in
+           (one : one_inductive_body) : TemplateMonad (BasicAst.def named_term) :=
+  let this_name := nNamed ("$rep" ++ string_of_nat (inductive_ind ind)) in
   prop <- matchmaker ind one tau (process_ctors (ind_ctors one)) ;;
   let body :=
-      (tLambda (nNamed "$g"%string) <% graph %>
-        (tLambda (nNamed "$x"%string) tau
-          (tLambda (nNamed "$p"%string) <% mtype %> prop))) in
-  ret {| dname := this_name
-       ; dtype := tProd (nNamed "$g"%string)
+      (tLambda (mkBindAnn (nNamed "$g") Relevant) <% graph %>
+        (tLambda (mkBindAnn (nNamed "$x") Relevant) tau
+          (tLambda (mkBindAnn (nNamed "$p") Relevant) <% mtype %> prop))) in
+  ret {| dname := mkBindAnn this_name Relevant
+       ; dtype := tProd (mkBindAnn (nNamed "$g") Relevant)
                        <% graph %>
-                       (tProd (nNamed "$x"%string)
+                       (tProd (mkBindAnn (nNamed "$x") Relevant)
                                tau
-                               (tProd (nNamed "$p"%string)
+                               (tProd (mkBindAnn (nNamed "$p") Relevant)
                                      <% mtype %>
                                      <% Prop %>))
        ; dbody := body
        ; rarg := 1 |}.
 
 (* Remove all the initial consecutive π-type quantifiers from a [term]. *)
-Fixpoint strip_quantifiers (t : term) : term :=
+Fixpoint strip_quantifiers (t : named_term) : named_term :=
   match t with
   | tProd _ _ rest => strip_quantifiers rest
   | x => x
   end.
 
 (* Get binder names and binding types for all
-   initial consecutive π-type quantifiers in a [term]. *)
-Fixpoint get_quantifiers (t : term) : list (name * term) :=
+   initial consecutive π-type quantifiers in an [any_term]. *)
+Fixpoint get_quantifiers
+         (modify : ident -> ident)
+         (t : any_term) : list (aname * any_term) :=
   match t with
-  | tProd n ty rest => (n, ty) :: get_quantifiers rest
+  | tProd (mkBindAnn nAnon rel) ty rest =>
+    (mkBindAnn nAnon rel, ty) :: get_quantifiers modify rest
+  | tProd (mkBindAnn (nNamed id) rel) ty rest =>
+    (mkBindAnn (nNamed (modify id)) rel, ty) :: get_quantifiers modify rest
   | x => nil
   end.
 
-(* Given binder names and binding types, add binders to the base [term].
+(* Given binder names and binding types, add binders to the base [named_term].
    Can be used to add λs (with [tLambda]) or πs (with [tProd]). *)
 Fixpoint build_quantifiers
-         (binder : name -> term -> term -> term)
-         (l : list (name * term))
-         (base : term) : term :=
+         (binder : aname -> named_term -> named_term -> named_term)
+         (l : list (aname * named_term))
+         (base : named_term) : named_term :=
   match l with
   | nil => base
   | (n, t) :: rest => binder n t (build_quantifiers binder rest base)
@@ -431,9 +611,13 @@ Definition add_instances (kn : kername) : TemplateMonad unit :=
                (fun i one =>
                   (* FIXME get rid of repeated computation here *)
                   let ind := {| inductive_mind := kn ; inductive_ind := i |} in
-                  quantified <- generate_instance_type ind one id ;;
-                  quantified_named <- DB.undeBruijn [] quantified ;;
-                  let tau := strip_quantifiers quantified_named in
+                  quantified <- generate_instance_type ind one
+                                  (fun ty_name t =>
+                                    let n := "$Rep_" ++ Prototype.remove_sigils' ty_name in
+                                    tProd (mkBindAnn (nNamed n) Relevant) (tApp <% Rep %> [tVar ty_name]) t)
+                                    id ;;
+                  (* quantified_named <- DB.undeBruijn [] quantified ;; *)
+                  let tau := strip_quantifiers quantified in
                   make_fix_single tau {| inductive_mind := kn ; inductive_ind := i |} one)
                (ind_bodies mut) ;;
 
@@ -443,39 +627,59 @@ Definition add_instances (kn : kername) : TemplateMonad unit :=
        let ind := {| inductive_mind := kn ; inductive_ind := i |} in
        (* This gives us something like
           [forall (A : Type) (n : nat), vec A n] *)
-       quantified <- generate_instance_type ind one id ;;
+       quantified <- generate_instance_type ind one
+                      (fun ty_name t =>
+                        let n := "$Rep_" ++ Prototype.remove_sigils' ty_name in
+                        tProd (mkBindAnn (nNamed n) Relevant) (tApp <% Rep %> [tVar ty_name]) t)
+                      id ;;
+       tmMsg "quantified:" ;;
+       tmEval all quantified >>= tmPrint ;;
+
        (* Now what can we do with this?
           Let's start by going to its named representation. *)
-       quantified_named <- DB.undeBruijn [] quantified ;;
+       (* quantified_named <- DB.undeBruijn [] quantified ;; *)
 
+       (* tmEval all quantified_named >>= tmPrint ;; *)
        (* The reified type of the fully applied type constructor,
           but with free variables! *)
-       let tau := strip_quantifiers quantified_named in
-       let fn_ty := tProd (nNamed "$g"%string)
+       let tau := strip_quantifiers quantified in
+       let fn_ty := tProd (mkBindAnn (nNamed "$g") Relevant)
                           <% graph %>
-                          (tProd (nNamed "$x"%string)
+                          (tProd (mkBindAnn (nNamed "$x") Relevant)
                                  tau
-                                 (tProd (nNamed "$p"%string)
+                                 (tProd (mkBindAnn (nNamed "$p") Relevant)
                                         <% mtype %>
                                         <% Prop %>)) in
-       let quantifiers := get_quantifiers quantified_named in
-       let prog_named : term :=
+       let quantifiers : list (aname * any_term) :=
+           get_quantifiers id quantified in
+           (* get_quantifiers (fun id => "$" ++ id) quantified_named in *)
+       let prog_named : named_term :=
            build_quantifiers tLambda quantifiers
-                             (tApp (tConstruct {| inductive_mind := <? Rep ?>
-                                                ; inductive_ind := 0 |} 0 [])
+                             (tApp <% @Build_Rep %>
                                    [tau; tFix singles i]) in
+       tmMsg "" ;;
+       tmMsg "Final:" ;;
+       tmEval all prog_named >>= tmPrint ;;
 
        (* Convert generated program from named to de Bruijn representation *)
        prog <- DB.deBruijn prog_named ;;
+       tmMsg "Final unnamed:" ;;
+       tmEval all prog >>= tmPrint ;;
 
+       extra_quantified <- DB.deBruijn (build_quantifiers tProd quantifiers
+                                                          (tApp <% Rep %> [tau])) ;;
+       tmMsg "Instance ty before:" ;;
+       tmEval all extra_quantified >>= tmPrint ;;
        (* If need be, here's the reified type of our [Rep] instance: *)
-       (*    instance_ty <-
-               tmUnquoteTyped Type
-                 (build_quantifiers tProd quantifiers
-                                   (tApp <% Rep %> [quantified])) ;;
-       *)
+       instance_ty <- tmUnquoteTyped Type extra_quantified ;;
+
+       tmMsg "Instance ty:" ;;
+       tmEval all instance_ty >>= tmPrint ;;
 
        instance <- tmUnquote prog ;;
+
+       tmMsg "Instance:" ;;
+       tmEval all instance >>= tmPrint ;;
        (* Remove [tmEval] when MetaCoq issue 455 is fixed: *)
        (* https://github.com/MetaCoq/metacoq/issues/455 *)
        name <- tmFreshName =<< tmEval all ("Rep_" ++ ind_name one)%string ;;
@@ -504,23 +708,124 @@ Definition add_instances (kn : kername) : TemplateMonad unit :=
        ret tt) (ind_bodies mut) ;;
   ret tt.
 
-(* Derives a [Rep] instance for the type constructor [Tau] *)
-(*    and the types its definition depends on. *)
+(* Derives a [Rep] instance for the type constructor [Tau],
+   and the types its definition depends on. *)
 Definition rep_gen {kind : Type} (Tau : kind) : TemplateMonad unit :=
   '(env, tau) <- tmQuoteRec Tau ;;
   missing <- find_missing_instances env ;;
   monad_iter add_instances (rev missing).
 
 
-(* Let's see it in action: *)
 
-MetaCoq Run (rep_gen bool).
-Print Rep_bool.
+(* Playground: *)
+MetaCoq Run (rep_gen nat).
+Print Rep_nat.
+
+Inductive T (A : Type):=
+| C : A -> T A.
+MetaCoq Run (rep_gen T).
+MetaCoq Run (rep_gen list).
+
+Inductive fin : nat -> Set :=
+| F1 : forall {n}, fin (S n)
+| FS : forall {n}, fin n -> fin (S n).
+
+(* MetaCoq Run (rep_gen fin). *)
+
+
+(* Instance Rep_nat : Rep nat := *)
+(*   {| rep _ _ _ := False |}. *)
+(* Instance Rep_list {A} `{Rep A} : Rep (list A) := *)
+(*   {| rep _ _ _ := False |}. *)
+
+(* Check <% forall A `{Rep A}, Rep (list A)%>. *)
+(* Check <% forall A, Rep A -> Rep (list A)%>. *)
+(* MetaCoq Run (o <- tmInferInstance (Some all) (forall A, Rep A -> Rep (list A)) ;; *)
+(*              tmPrint o). *)
+
+
+
+
+Check <%% le %%>.
+(* Let's see it in action: *)
+MetaCoq Run (rep_gen unit).
+Print Rep_unit.
+(* fitting_index g p (enum 0) [] *)
+
+(* MetaCoq Run (rep_gen bool). *)
+(* Print Rep_bool. *)
+
+Print name.
+Check <%% list %%>.
+
+Inductive T (n : nat) (eq : n = 0) : nat -> Type :=
+| C : T n eq (n + n).
+
+Instance Rep_T n eq n' : Rep (T n eq n') :=
+  {| rep g x p :=
+       match x with
+       | C => False
+       end
+  |}.
+
+Check <%% T %%>.
+Check (fun (t : T 0 (eq_refl 0) 0) => match t with C => true end).
+
+Fixpoint rep0 (g : graph) (x : nat) (p : mtype) {struct x} : Prop :=
+  match x with
+  | 0 => fitting_index g p (enum 0) []
+  | S arg0 =>
+      exists p0 : mtype, rep0 g arg0 p0 /\ fitting_index g p (boxed 0 1) [p0]
+  end.
+Instance Rep_nat : Rep nat := @Build_Rep nat rep0.
 
 MetaCoq Run (rep_gen nat).
 Print Rep_nat.
 
-(* MetaCoq Run (rep_gen list). *)
+Inductive vec (A : Type) : nat -> Type :=
+| vnil : vec A O
+| vcons : forall n, A -> vec A n -> vec A (S n).
+
+Instance Rep_vec (A : Type) (Rep_A : Rep A) (n : nat) : Rep (vec A n) :=
+  let fix rep_vec (n : nat) (g : graph) (x : vec A n) (p : mtype) {struct x} : Prop :=
+    match x with
+    | vnil => fitting_index g p (enum 0) []
+    | vcons arg0 arg1 arg2 =>
+        exists p0 p1 p2 : mtype,
+          @rep nat Rep_nat g arg0 p0 /\
+          @rep A Rep_A g arg1 p1 /\
+          rep_vec arg0 g arg2 p2 /\
+          fitting_index g p (boxed 0 3) [p0; p1; p2]
+    end
+  in @Build_Rep (vec A n) (rep_vec n).
+
+Inductive fin : nat -> Set :=
+| F1 : forall {n}, fin (S n)
+| FS : forall {n}, fin n -> fin (S n).
+
+Check <%% fin %%>.
+
+(* Inductive T (x : unit) : Type := *)
+(* | C : T x. *)
+(* Check <%% T %%>. *)
+MetaCoq Run (rep_gen fin').
+(* Print Rep_fin'. *)
+
+Instance Rep_fin (n : nat) : Rep (fin n) :=
+  let fix rep_fin (n : nat) (g : graph) (x : fin n) (p : mtype) {struct x} : Prop :=
+    match x with
+    | @F1 arg0 =>
+        exists p0 : mtype, rep g arg0 p0 /\ fitting_index g p (boxed 0 1) [p0]
+    | @FS arg0 arg1 =>
+        exists p0 p1 : mtype,
+          rep g arg0 p0 /\
+          rep_fin arg0 g arg1 p1 /\ fitting_index g p (boxed 1 2) [p0; p1]
+    end in @Build_Rep (fin n) (rep_fin n).
+
+MetaCoq Run (rep_gen fin).
+(* Print Rep_fin. *)
+
+MetaCoq Run (rep_gen list).
 (* Print Rep_list. *)
 
 Inductive rgx : Type :=
@@ -531,23 +836,23 @@ Inductive rgx : Type :=
 | and     : rgx -> rgx -> rgx
 | star    : rgx -> rgx.
 
-MetaCoq Run (rep_gen rgx).
-Print Rep_rgx.
+(* MetaCoq Run (rep_gen rgx). *)
+(* Print Rep_rgx. *)
 
 Inductive R1 :=
 | r1 : R1
 with R2 :=
 | r2 : R2.
 
-MetaCoq Run (rep_gen R1).
-Print Rep_R1.
+(* MetaCoq Run (rep_gen R1). *)
+(* Print Rep_R1. *)
 
 Inductive T1 :=
 | c1 : T2 -> T1
 with T2 :=
 | c2 : T1 -> T2.
 
-(* MetaCoq Run (rep_gen T1). *)
+MetaCoq Run (rep_gen T1).
 (* Print Rep_T1. *)
 
 Inductive param_and_index (a b : nat) : a < b -> Type :=
@@ -561,3 +866,33 @@ Inductive indexed : nat -> Type :=
 
 (* MetaCoq Run (rep_gen indexed). *)
 (* Print Rep_indexed. *)
+
+
+(* "Haskell Programming with Nested Types: A Principled Approach", Johann and Ghani, 2009 *)
+Inductive lam (A : Type) : Type :=
+| variable : A -> lam A
+| app : lam A -> lam A -> lam A
+| abs : lam (option A) -> lam A.
+
+
+Inductive digit (A : Type) : Type :=
+| one : A -> digit A
+| two : A -> A -> digit A
+| three : A -> A -> A -> digit A
+| four : A -> A -> A -> A -> digit A.
+Inductive node (A : Type) : Type :=
+| node2 : nat -> A -> A -> node A
+| node3 : nat -> A -> A -> A -> node A.
+Inductive finger_tree (A : Type) : Type :=
+| emptyT : finger_tree A
+| single : A -> finger_tree A
+| deep : nat -> digit A -> finger_tree (node A) -> digit A -> finger_tree A.
+
+
+Inductive two (A : Type) := mkTwo : A -> A -> two A.
+Inductive tree (A : Type) : Type :=
+| leaf : tree A
+| node : two (tree A) -> tree A.
+Inductive ntree (A : Type) : Type :=
+| nleaf : ntree A
+| nnode : ntree (two A) -> ntree A.
